Added ex06 solution

test01/20-11-2019/6.dfy
@@ -11,10 +11,20 @@ trait Node {
    var child: set<Node>; 
 
     predicate Valid() {
-        // TODO
+        //(i)names of child nodes are unique (no duplicates) 
+        forall x, y :: x in child && y in child && x != y ==> x.name != y.name
+        //(ii)the depth of child nodes is the depth of this node plus one
+        && forall children :: children in child ==> children.depth == this.depth + 1
     }
 
-     constructor (name: string, parent: Folder?) {
+     constructor (name: string, parent: Folder?)
+        modifies parent
+        requires |name| > 0
+        ensures this.name == name
+        ensures this.child == {}
+        ensures parent != null ==> parent.child == parent.child + {this} && this.depth == parent.depth + 1
+        ensures parent == null ==> this.depth == 0
+    {
        // this object initialization
         this.name := name;
         this.depth := if parent == null then 0 else parent.depth + 1;
